src/circuit2.v
@@ -1,0 +1,86 @@
+From research Require Import base.
+From research Require Export action.
+From stdpp Require Import option.
+
+Class Circuit (s m tr : Type) :=
+  { mkCircuit : s
+  ; circuitCall : m -> @Action s unit
+  ; circuitTrace : s -> list tr
+  }.
+
+Definition circuitStep `(c : Circuit s m tr) (method : m) (state : s) : s :=
+  nextState (circuitCall method) state.
+
+Definition circuitSteps `(c : Circuit s m tr) (ms : list m) (state : s) : s :=
+  fold_left (fun st m => circuitStep c m st) ms state.
+
+Definition runCircuit `(c : Circuit s m tr) (ms : list m) : s :=
+  circuitSteps c ms mkCircuit.
+
+Lemma circuitStepsApp `(c: Circuit s m tr) : forall xs1 xs2 st,
+    circuitSteps c (xs1 ++ xs2) st =
+      circuitSteps c xs2 (circuitSteps c xs1 st).
+Proof.
+  cbv [circuitSteps].
+  intros ???.
+  rewrite fold_left_app.
+  equality.
+Qed.
+
+Lemma runCircuitApp `(c: Circuit s m tr) : forall xs1 xs2,
+    runCircuit c (xs1 ++ xs2) =
+      circuitSteps c xs2 (runCircuit c xs1).
+Proof.
+  cbv [runCircuit].
+  intros ??.
+  apply circuitStepsApp.
+Qed.
+
+Definition simulates {s1 s2 t1 t2} a1 a2 (R : s1 -> s2 -> Prop) :=
+  forall st1 st2,
+    R st1 st2 ->
+    (forall st1' st2',
+        st1' = nextState (a := t1) a1 st1 ->
+        st2' = nextState (a := t2) a2 st2 ->
+        R st1' st2').
+
+Notation "m1 ⪯ m2 : R" := (simulates m1 m2 R) (at level 60, m2 at next level).
+
+Definition circuitSimulates `(c1: Circuit s1 m1 tr) `(c2: Circuit s2 m2 tr) p R
+  := forall m, c1.(circuitCall) m ⪯ c2.(circuitCall) (p m) : R.
+
+Notation "c1 ∼ c2 : policy ; R" :=
+  (circuitSimulates c1 c2 policy R) (at level 60, c2 at next level).
+
+(* We say a circuit [c] is constant time relevant to some policy [policy],
+   if given the set of method calls to [c], we get the specification leakage
+   by applying policy [policy] to the series of method calls. If from the specification
+   leakage we can determine the implementation leakage trace, we get constant time
+   wrt [policy]. *)
+Definition constantTime {m2} `(c : Circuit s m1 tr) (policy : list m1 -> list m2) :=
+  exists f, forall xs, circuitTrace (runCircuit c xs) = f (policy xs).
+
+Lemma circuitConstantTime
+  `(c1 : Circuit s1 m1 tr)
+  `(c2 : Circuit s2 m2 tr) policy :
+  forall R, (c1 ∼ c2 : policy; R) ->
+       R c1.(mkCircuit) c2.(mkCircuit) ->
+       (forall st1 st2, R st1 st2 -> c1.(circuitTrace) st1 = c2.(circuitTrace) st2) ->
+       constantTime c1 (map policy).
+Proof.
+  intros R Hsimulates Hinit Htrace.
+  cbv [ constantTime circuitSimulates simulates ] in *.
+  exists (fun zs => circuitTrace (runCircuit c2 zs)).
+  intros.
+  apply Htrace.
+  induction xs using rev_ind.
+  - assumption.
+  - rewrite map_app.
+    rewrite !runCircuitApp.
+    simplify.
+    set (st1 := runCircuit c1 xs) in *.
+    set (st2 := runCircuit c2 (map policy xs)) in *.
+    apply Hsimulates with (st1 := st1) (st2 := st2) (m := x); equality.
+Qed.
+
+Arguments Circuit {_ _ _}.
